coq/apex.v
@@ -222,17 +222,12 @@ Lemma trace_pure et l1 l2:
   kind et == T -> ~~ has (matchingMA et) l2 -> p = l1 ++ et :: l2 -> 
   source et # fld et = new et.
 Proof.
-move=>Kt; elim:l2=>[_|].
-
-rewrite cats1=>Z; subst p.
-have er: {er : ExecuteResult | executeLog g0 l1 = Some er}
-  by apply: replayLogRcons; apply: (exist _ _ epf).
-case:er=>[[h' g']]pf'.
-
-
-
-
-Qed.
+(* move=>Kt; elim:l2=>[_|]. *)
+(* rewrite cats1=>Z; subst p. *)
+(* have er: {er : ExecuteResult | executeLog g0 l1 = Some er} *)
+(*   by apply: replayLogRcons; apply: (exist _ _ epf). *)
+(* case:er=>[[h' g']]pf'. *)
+Admitted.
 
 (* [TODO] The next step is prove that for any T-entry, its captured
    o.f-value is either in the graph, or there exists an MA-antry *behind*
@@ -248,23 +243,11 @@ Lemma traced_objects et l1 l2 :
   o#f = n \/
   has (fun ema => (matchingMA et ema) && (o#f == new ema)) l2.
 Proof.
-move=>/=E Kt.
-case X: (has (matchingMA et) l2); last first; [left | right].
-
-move/negbT: X=>/hasPn.
-
-Search _ (has _).
-
-
-
-  
-
-
-(* The following subfacts should be proved:
-  
-
-
- *)
+(* move=>/=E Kt. *)
+(* case X: (has (matchingMA et) l2); last first; [left | right]. *)
+(* move/negbT: X=>/hasPn. *)
+(* Search _ (has _). *)
+Admitted.
 
 
 
